rocq/theories/TypeSystem/EnvRootSoundness.v
@@ -538,9 +538,9 @@ Proof.
 	      inversion Hinfer; subst.
 	      destruct (lookup_fn_b_sound i (env_fns env) fdef Hlookup) as [Hin Hname].
 	      eapply TER_Fn; eassumption.
-	    + destruct (lookup_fn_b i (env_fns env)) as [fdef |] eqn:Hlookup; try discriminate.
-	      destruct (check_make_closure_captures_sctx env Ω Σ l (fn_captures fdef))
-	        as [captured_tys | err] eqn:Hcheck; try discriminate.
+		    + destruct (lookup_fn_b i (env_fns env)) as [fdef |] eqn:Hlookup; try discriminate.
+		      destruct (check_make_closure_captures_sctx_with_env env Ω Σ l (fn_captures fdef))
+		        as [[env_lt captured_tys] | err] eqn:Hcheck; try discriminate.
 	      inversion Hinfer; subst.
 	      destruct (lookup_fn_b_sound i (env_fns env) fdef Hlookup) as [Hin Hname].
 	      eapply TER_MakeClosure; eassumption.
@@ -836,9 +836,9 @@ Proof.
 	      inversion Hinfer; subst.
 	      destruct (lookup_fn_b_sound i (env_fns env) fdef Hlookup) as [Hin Hname].
 	      eapply TERS_Fn; eassumption.
-	    + destruct (lookup_fn_b i (env_fns env)) as [fdef |] eqn:Hlookup; try discriminate.
-	      destruct (check_make_closure_captures_sctx env Ω Σ l (fn_captures fdef))
-	        as [captured_tys | err] eqn:Hcheck; try discriminate.
+		    + destruct (lookup_fn_b i (env_fns env)) as [fdef |] eqn:Hlookup; try discriminate.
+		      destruct (check_make_closure_captures_sctx_with_env env Ω Σ l (fn_captures fdef))
+		        as [[env_lt captured_tys] | err] eqn:Hcheck; try discriminate.
 	      inversion Hinfer; subst.
 	      destruct (lookup_fn_b_sound i (env_fns env) fdef Hlookup) as [Hin Hname].
 	      eapply TERS_MakeClosure; eassumption.
